`LGS.v`: `Module Rule`.

theories/System/LGS.v
@@ -101,7 +101,7 @@ Inductive t : Set :=
 End BuildError.
 
 #[universes(polymorphic=yes)]
-Definition BuildErrorM@{u} (A : Type@{u}) : Type@{u} :=
+Definition BuildErrorM@{u | } (A : Type@{u}) : Type@{u} :=
   BuildError.t + A.
 
 #[universes(polymorphic=yes)]
@@ -142,8 +142,326 @@ Qed.
 #[local] Existing Instance list_corresponds_to_finite_ensemble.
 #[local] Existing Instance alist_corresponds_to_finite_partial_map.
 
-Module LGS (Token : TOKEN_SPEC).
+Module MkLGS (Token : TOKEN_SPEC).
 
 #[global] Existing Instance Token.t_hasEqDec.
 
-End LGS.
+Module Input.
+
+Definition t : Set :=
+  list ascii.
+
+Fixpoint of_string (s : string) : Input.t :=
+  match s with
+  | EmptyString => []
+  | String c s' => c :: of_string s'
+  end.
+
+Fixpoint to_string (s : Input.t) : string :=
+  match s with
+  | [] => EmptyString
+  | c :: s' => String c (to_string s')
+  end.
+
+Theorem to_of_string (s : string)
+  : to_string (of_string s) = s.
+Proof.
+  induction s as [ | c s IH]; simpl; congruence.
+Qed.
+
+Theorem of_to_string (s : Input.t)
+  : of_string (to_string s) = s.
+Proof.
+  induction s as [ | c s IH]; simpl; congruence.
+Qed.
+
+Theorem length_of_string (s : string)
+  : length (of_string s) = String.length s.
+Proof.
+  induction s as [ | c s IH]; simpl; congruence.
+Qed.
+
+Theorem to_string_app (s1 : Input.t) (s2 : Input.t)
+  : to_string (s1 ++ s2) = String.append (to_string s1) (to_string s2).
+Proof.
+  induction s1 as [ | c s1 IH]; simpl; congruence.
+Qed.
+
+Theorem prefix_suffix_decompose (s : Input.t) (n : nat)
+  (LE : n <= length s)
+  : exists prefix, exists suffix, s = prefix ++ suffix /\ length prefix = n.
+Proof.
+  exists (firstn n s), (skipn n s).
+  rewrite firstn_skipn. split; [reflexivity | ].
+  rewrite length_firstn. lia.
+Qed.
+
+Theorem app_cancel_prefix (prefix : Input.t) (s1 : Input.t) (s2 : Input.t)
+  (EQ : prefix ++ s1 = prefix ++ s2)
+  : s1 = s2.
+Proof.
+  eapply L.app_cancel_l. exact EQ.
+Qed.
+
+Theorem app_cancel_suffix (s1 : Input.t) (s2 : Input.t) (suffix : Input.t)
+  (EQ : s1 ++ suffix = s2 ++ suffix)
+  : s1 = s2.
+Proof.
+  eapply L.app_cancel_r. exact EQ.
+Qed.
+
+Theorem empty_or_nonempty (s : Input.t)
+  : s = [] \/ (exists c, exists s', s = c :: s').
+Proof.
+  destruct s as [ | c s']; [left; reflexivity | right; exists c, s'; reflexivity].
+Qed.
+
+Theorem nonempty_prefix_rest_shorter (consumed : Input.t) (rest : Input.t)
+  (NONEMPTY : ~ consumed = [])
+  : length rest < length (consumed ++ rest).
+Proof.
+  destruct consumed as [ | c consumed]; [contradiction | simpl; rewrite length_app; simpl; lia].
+Qed.
+
+End Input.
+
+Lemma Input_to_of_string (s : string)
+  : Input.to_string (Input.of_string s) = s.
+Proof.
+  induction s as [ | c s IH]; simpl; congruence.
+Qed.
+
+Lemma Input_of_to_string (s : Input.t)
+  : Input.of_string (Input.to_string s) = s.
+Proof.
+  induction s as [ | c s IH]; simpl; congruence.
+Qed.
+
+Lemma Input_length_of_string (s : string)
+  : length (Input.of_string s) = String.length s.
+Proof.
+  induction s as [ | c s IH]; simpl; congruence.
+Qed.
+
+Lemma Input_to_string_app (s1 : Input.t) (s2 : Input.t)
+  : Input.to_string (s1 ++ s2) = String.append (Input.to_string s1) (Input.to_string s2).
+Proof.
+  induction s1 as [ | c s1 IH]; simpl; congruence.
+Qed.
+
+Fixpoint nullable (e : regex ascii) {struct e} : bool :=
+  match e with
+  | Re.Null => false
+  | Re.Empty => true
+  | Re.Char c => false
+  | Re.Union e1 e2 => nullable e1 || nullable e2
+  | Re.Append e1 e2 => nullable e1 && nullable e2
+  | Re.Star e1 => true
+  end.
+
+Lemma nullable_similar_spec (e : regex ascii)
+  : nullable e = true <-> [] =~= e.
+Proof.
+  split.
+  - induction e as [ | | c | e1 IH1 e2 IH2 | e1 IH1 e2 IH2 | e IH]; simpl; i; try congruence.
+    + econs.
+    + rewrite orb_true_iff in H. destruct H as [H | H]; eauto with *.
+    + rewrite andb_true_iff in H. destruct H as [H1 H2].
+      change (@nil ascii) with (@nil ascii ++ @nil ascii).
+      eauto with *.
+    + econs.
+  - revert e.
+    enough (CLAIM : forall s, forall e, s =~= e -> s = [] -> nullable e = true).
+    { i. eapply CLAIM; eauto. }
+    intros s e H_IN. induction H_IN; simpl; i; subst; try congruence; eauto.
+    + rewrite orb_true_iff. left. eauto.
+    + rewrite orb_true_iff. right. eauto.
+    + pose proof (app_eq_nil _ _ H) as [EQ1 EQ2]. subst s1 s2. ss!.
+Qed.
+
+Theorem nullable_true_iff (e : regex ascii)
+  : nullable e = true <-> [] \in eval_regex e.
+Proof.
+  rewrite eval_regex_good. eapply nullable_similar_spec.
+Qed.
+
+Theorem nullable_false_iff (e : regex ascii)
+  : nullable e = false <-> (~ [] \in eval_regex e).
+Proof.
+  destruct (nullable e) eqn: EQ; split; intros H.
+  - congruence.
+  - contradiction H. rewrite <- nullable_true_iff. exact EQ.
+  - intros IN. rewrite <- nullable_true_iff in IN. congruence.
+  - reflexivity.
+Qed.
+
+Corollary nullable_refines (e : regex ascii)
+  : nullable e ⊑ ([] \in eval_regex e).
+Proof.
+  destruct (nullable e) as [ | ] eqn: H_OBS.
+  - now rewrite nullable_true_iff in H_OBS.
+  - now rewrite nullable_false_iff in H_OBS.
+Qed.
+
+Lemma union_inv (s : Input.t) (e1 : regex ascii) (e2 : regex ascii)
+  (IN : s \in eval_regex (Re.Union e1 e2))
+  : s \in eval_regex e1 \/ s \in eval_regex e2.
+Proof.
+  done!.
+Qed.
+
+Lemma append_inv (s : Input.t) (e1 : regex ascii) (e2 : regex ascii)
+  (IN : s \in eval_regex (Re.Append e1 e2))
+  : exists s1, exists s2, s = s1 ++ s2 /\ s1 \in eval_regex e1 /\ s2 \in eval_regex e2.
+Proof.
+  done!.
+Qed.
+
+Lemma star_nil (e : regex ascii)
+  : [] \in eval_regex (Re.Star e).
+Proof.
+  econs 1.
+Qed.
+
+Theorem star_inv (s : Input.t) (e : regex ascii)
+  (IN : s \in eval_regex (Re.Star e))
+  : s = [] \/ (exists s1, exists s2, s = s1 ++ s2 /\ s1 \in eval_regex e /\ s2 \in eval_regex (Re.Star e)).
+Proof.
+  simpl in IN. inv IN; [left | right]; ss!.
+Qed.
+
+Module Rule.
+
+#[projections(primitive)]
+Record t : Set :=
+  mk
+  { index : nat
+  ; token : Token.t
+  ; regex : Re.t ascii
+  } as rule.
+
+#[global]
+Instance Rule_hasEqDec
+  : hasEqDec@{Set} Rule.t.
+Proof.
+  red; decide equality; eapply eq_dec.
+Defined.
+
+Definition compileRule (rule : Rule.t) : BuildErrorM Rule.t :=
+  if nullable rule.(Rule.regex) then
+    inl (BuildError.NullableTokenRule rule.(Rule.index))
+  else
+    pure rule.
+
+Theorem compileRule_spec (rule : Rule.t) (rule' : Rule.t)
+  (COMPILE : compileRule rule = inr rule')
+  : forall s, s \in eval_regex rule.(Rule.regex) <-> s \in eval_regex rule'.(Rule.regex).
+Proof.
+  intros s; split; intros ACCEPTS; unfold compileRule in COMPILE; now destruct (nullable rule.(Rule.regex)) eqn: NULLABLE; inv COMPILE.
+Qed.
+
+Lemma compileRule_not_match_empty (rule : Rule.t) (rule' : Rule.t)
+  (COMPILE : compileRule rule = inr rule')
+  : ~ ([] \in eval_regex rule'.(Rule.regex)).
+Proof.
+  unfold compileRule in COMPILE; destruct (nullable rule.(Rule.regex)) eqn: NULLABLE; inv COMPILE; now rewrite <- nullable_false_iff.
+Qed.
+
+Fixpoint compileRules (rules : list Rule.t) : BuildErrorM (list Rule.t) :=
+  match rules with
+  | [] => pure (@nil Rule.t)
+  | rule :: rules => liftM2 (@cons Rule.t) (compileRule rule) (compileRules rules)
+  end.
+
+Definition raws : list Rule.t :=
+  L.mapi_from 1 (fun index => fun '(token, regex) => Rule.mk index token regex) Token.rules.
+
+Definition compileds : BuildErrorM (list Rule.t) :=
+  compileRules raws.
+
+Definition accepts (rule : Rule.t) (s : Input.t) : Prop :=
+  s \in eval_regex rule.(Rule.regex).
+
+Definition first_rule_for (rules : list Rule.t) (s : Input.t) (rule : Rule.t) : Prop :=
+  exists prefix, exists suffix, rules = prefix ++ rule :: suffix /\ accepts rule s /\ (forall prior, prior ∈ prefix -> ~ accepts prior s).
+
+Definition priority (rules : list Rule.t) (rule1 : Rule.t) (rule2 : Rule.t) : Prop :=
+  exists between, exists suffix, rules = rule1 :: between ++ rule2 :: suffix.
+
+Lemma compileRule_success_identity (rule : Rule.t) (rule' : Rule.t)
+  (COMPILE : compileRule rule = inr rule')
+  : rule = rule'.
+Proof.
+  unfold compileRule in *. now destruct (nullable rule.(Rule.regex)); inv COMPILE.
+Qed.
+
+Lemma compileRules_preserve_order (rules : list Rule.t) (rules' : list Rule.t)
+  (COMPILE : compileRules rules = inr rules')
+  : rules = rules'.
+Proof.
+  revert rules' COMPILE; induction rules as [ | rule rules IH]; intros compiled_rules COMPILE; simpl in COMPILE.
+  - now inv COMPILE.
+  - destruct (compileRule rule) as [err | rules'] eqn: COMPILE_RULE; cbn in COMPILE; [discriminate | ].
+    destruct (compileRules rules) as [err | compiled_rules']; cbn in COMPILE; [discriminate | ].
+    inv COMPILE. f_equal.
+    + now eapply compileRule_success_identity.
+    + now eapply IH.
+Qed.
+
+Theorem compileRules_sound (rules : list Rule.t) (rules' : list Rule.t) (rule : Rule.t)
+  (COMPILE : compileRules rules = inr rules')
+  (IN : rule ∈ rules')
+  : rule ∈ rules /\ (~ accepts rule []).
+Proof.
+  split.
+  - revert rule rules' COMPILE IN; induction rules as [ | rule rules IH]; ii; simpl in *.
+    + now inv COMPILE.
+    + destruct (compileRule rule) as [err | rule'] eqn: H_OBS1; simpl in *; inv COMPILE.
+      destruct (compileRules rules) as [err | rules0] eqn: H_OBS2; simpl in *; inv H0.
+      destruct IN as [EQ | IN]; [left | right]; eauto.
+      eapply compileRule_success_identity. congruence.
+  - revert rule rules' COMPILE IN; induction rules as [ | rule rules IH]; ii; simpl in *.
+    + now inv COMPILE.
+    + destruct (compileRule rule) as [err | rule'] eqn: H_OBS1; simpl in *; inv COMPILE.
+      destruct (compileRules rules) as [err | rules0] eqn: H_OBS2; simpl in *; inv H1.
+      destruct IN as [EQ | IN].
+      * eapply compileRule_not_match_empty with (rule := rule) (rule' := rule0); eauto. congruence.
+      * eapply IH with (rule := rule0) (rules' := rules0); eauto.
+Qed.
+
+Theorem compileRules_complete (rules : list Rule.t)
+  (NONNULL : forall rule, rule ∈ rules -> nullable rule.(Rule.regex) = false)
+  : compileRules rules = inr rules.
+Proof.
+  induction rules as [ | rule rules IH]; simpl; eauto.
+  unfold compileRule at 1. rewrite NONNULL by now left.
+  cbn. rewrite IH; ss!.
+Qed.
+
+Theorem compileRules_failure_nullable (rules : list Rule.t) (err : BuildError.t)
+  (COMPILE : compileRules rules = inl err)
+  : exists rule, rule ∈ rules /\ nullable rule.(Rule.regex) = true /\ err = BuildError.NullableTokenRule rule.(Rule.index).
+Proof.
+  revert err COMPILE; induction rules as [ | rule rules IH]; intros err COMPILE; simpl in COMPILE; try congruence.
+  destruct (compileRule rule) as [err' | rule'] eqn: COMPILE_RULE; cbn in COMPILE.
+  - inv COMPILE. unfold compileRule in COMPILE_RULE. destruct (nullable rule.(Rule.regex)) eqn: NULLABLE; inv COMPILE_RULE. exists rule; ss!.
+  - destruct (compileRules rules) as [err' | rules'] eqn: COMPILE_RULES; cbn in COMPILE; try congruence.
+    inv COMPILE. pose proof (IH err eq_refl) as (bad_rule & IN_RULES & NULLABLE & ERR). exists bad_rule; ss!.
+Qed.
+
+Theorem compileRules_has_nullable_failure (rules : list Rule.t)
+  (NULLABLE : exists rule, rule ∈ rules /\ nullable rule.(Rule.regex) = true)
+  : exists idx, compileRules rules = inl (BuildError.NullableTokenRule idx).
+Proof.
+  induction rules as [ | rule rules IH].
+  - destruct NULLABLE as (bad_rule & [] & _).
+  - destruct NULLABLE as (bad_rule & [EQ | IN] & NULLABLE).
+    + subst bad_rule. simpl. unfold compileRule at 1. rewrite NULLABLE. ss!.
+    + simpl. destruct (compileRule rule) as [[idx] | compiled_rule] eqn: COMPILE_RULE; simpl; eauto.
+      pose proof (IH (@ex_intro _ _ bad_rule (conj IN NULLABLE))) as (idx & FAILURE); simpl.
+      rewrite FAILURE; exists idx; reflexivity.
+Qed.
+
+End Rule.
+
+End MkLGS.
